\documentclass[12pt]{book}
\usepackage[utf8]{inputenc}
\usepackage{color,soul,CJK,epic,tikz,array}
\usepackage{amsmath,amsthm,amssymb}
\setlength{\parindent}{0em}
\linespread{1.3}
\author{andersonwu2000}
\usepackage[margin=1cm]{geometry}
\pagestyle{empty}
\thispagestyle{empty} 

\newcounter{sect}

\newcounter{block}[sect]
\newenvironment{tblock}[1]
{\refstepcounter{block}\theblock.~\begin{minipage}[t]{\dimexpr\linewidth}#1\\}
{\end{minipage}\\}

\newenvironment{comm}
{\makebox[12pt][l]{$\bullet$}\begin{minipage}[t]{\dimexpr\linewidth}}
{\end{minipage}}

\begin{document}
\begin{CJK}{UTF8}{bsmi}

\hfill 章節 6-6 吳至堯 U10811023

%131 133 134 138

131. \begin{minipage}[t]{\dimexpr\linewidth}
Find the least squares approximation of $f(x)=x^2+2x$ over the interval $[0,2\pi]$ by \\
a. \begin{minipage}[t]{\dimexpr\linewidth}
a trigonometric polynomial of order 3 or less. \\
$\displaystyle f(x)\approx\frac{a_0}{2}+[a_1\cos x+a_2\cos2x]+[b_1\sin x+b_2\cos 2x]$ \\
$\displaystyle a_0=\frac{1}{\pi}\int_0^{2\pi}(x^2+2x)dx =
\left.\frac{x^3}{3\pi}+\frac{x^2}{\pi}\right|^{2\pi}_0 =
\frac{8\pi^2}{3}+4\pi$ \\
$\displaystyle a_k=\frac{1}{\pi}\int_0^{2\pi}(x^2+2x)\cos kxdx =
\frac{1}{\pi}\left(\int_0^{2\pi}x^2\cos kxdx+\int_0^{2\pi}2x\cos kxdx\right) = \frac{4}{k^2}$ \\
$\displaystyle b_k=\frac{1}{\pi}\int_0^{2\pi}(x^2+2x)\sin kxdx =
\frac{1}{\pi}\left(\int_0^{2\pi}x^2\sin kxdx+\int_0^{2\pi}2x\sin kxdx\right) = \frac{-4-4\pi}{k}$ \\
$\displaystyle\Rightarrow f(x)\approx\frac{4\pi^2}{3}+2\pi+4\cos x+\cos2x+(-4-4\pi)\sin x+(-2-2\pi)\sin2x$ \\
\end{minipage}
b. \begin{minipage}[t]{\dimexpr\linewidth}
a trigonometric polynomial of order n or less. \\
$\displaystyle f(x)\approx\frac{4\pi^2}{3}+2\pi+\sum_{r=1}^n\frac{4}{r^2}\cos rx+\sum_{s=1}^n\frac{-4-4\pi}{s}\sin sx$ \\
\end{minipage}
\end{minipage}\\

133.a. \begin{minipage}[t]{\dimexpr\linewidth}
Find the least squares approximation of $e^x$ over the interval $[0,1]$ by a function of the form $a_0+a_1x$ \\
$\Rightarrow$ basis of $a_0+a_1x : \textbf{u}_1=1,\textbf{u}_2=x\quad\Rightarrow\quad$Let $\displaystyle\textbf{v}_1=1,\textbf{v}_2=x-\frac{1\left\langle x, 1\right\rangle}{\parallel1\parallel^2}=x-\int_0^1x\ dx=x-\frac{1}{2}$ \\
$\Rightarrow$ orthonormal : Let $\displaystyle g_0=1,\  g_1=\frac{x-\frac{1}{2}}{\parallel x-\frac{1}{2}\parallel}=\frac{x-\frac{1}{2}}{\sqrt{\left\langle x-\frac{1}{2}, x-\frac{1}{2}\right\rangle}}=\frac{x-\frac{1}{2}}{\sqrt{\frac{1}{12}}}=2x\sqrt{3}-\sqrt{3}$ \\
$\Rightarrow\left\langle e^x, g_0\right\rangle g_0+\left\langle e^x, g_1\right\rangle g_1$ \begin{minipage}[t]{\dimexpr\linewidth}
$\displaystyle=\int_0^1e^x\ dx+\sqrt{3}(2x-1)\int_0^1\sqrt{3}e^x(2x-1)\ dx$ \\
$\displaystyle=e-1+3(2x-1)(\int_0^12xe^x\ dx-\int_0^1e^x\ dx)=-6ex+18x+4e-10$
\end{minipage}
\end{minipage}\\

133.b. \begin{minipage}[t]{\dimexpr\linewidth}
Find the mean square error of the approximation. \\
$\displaystyle\int_0^1[e^x+6ex-18x-4e+10]^2\ dx=\frac{1}{2}(-7e^2+40e-57)$
\end{minipage}\\

134.a. \begin{minipage}[t]{\dimexpr\linewidth}
Find the least squares approximation of $f(x)=\cos\pi x$ over the interval $[-1,1]$\\
by a function of the form $g(x)=a_0+a_1x+a_2x^2$ \\
$\Rightarrow$ basis of $a_0+a_1x+a_2x^2 : \textbf{u}_1=1,\textbf{u}_2=x,\textbf{u}_3=x^2$ \\
Let $\displaystyle
\textbf{v}_1=1,
\textbf{v}_2=x-\frac{1\left\langle x,1\right\rangle}{\parallel1\parallel^2}=x,
\textbf{v}_3=x^2-\frac{1\left\langle x^2,1\right\rangle}{\parallel1\parallel^2}-\frac{x\left\langle x^2,x\right\rangle}{\parallel x\parallel^2}=x^2-\frac{1}{3}$ \\
$\Rightarrow$ orthonormal : Let $\displaystyle g_0=\frac{1}{\parallel1\parallel}=\frac{1}{\sqrt{2}},\  g_1=\frac{x}{\parallel x\parallel}=\frac{x\sqrt{3}}{\sqrt{2}},\ g_2=\frac{x^2-\frac{1}{3}}{\parallel x^2-\frac{1}{3}\parallel}=\frac{(x^2-\frac{1}{3})\sqrt{45}}{\sqrt{8}}$ \\
$\Rightarrow$ \begin{minipage}[t]{\dimexpr\linewidth}
$\displaystyle=\left\langle \cos\pi x, g_0\right\rangle g_0+\left\langle \cos\pi x, g_1\right\rangle g_1+\left\langle \cos\pi x, g_2\right\rangle g_2$ \\
$\displaystyle=\frac{1}{\sqrt{2}}\int_{-1}^1\cos\pi x\ dx+\frac{\sqrt{3}}{\sqrt{2}}\int_{-1}^1x\cos\pi x\ dx+\frac{\sqrt{45}}{\sqrt{8}}\int_{-1}^1(x^2-\frac{1}{3})\cos\pi x\ dx=-\frac{6\sqrt{5}}{\pi^2\sqrt{2}}$
\end{minipage}
\end{minipage}\\

134.b. \begin{minipage}[t]{\dimexpr\linewidth}
Find the mean square error of the approximation. \\
$\displaystyle\int_{-1}^1[\cos\pi x+\frac{6\sqrt{5}}{\pi^2\sqrt{2}}]^2\ dx=1+\frac{180}{\pi^2}$
\end{minipage}\\

138. \begin{minipage}[t]{\dimexpr\linewidth}
Find the Fourier series of $f(x)=0,\ 0\le x<\pi$ and $f(x)=1,\ \pi\le x\le2\pi$ over the interval $[0, 2\pi]$ \\
$\displaystyle a_0=\frac{1}{\pi}\int_0^{2\pi}f(x)\ dx=\frac{1}{\pi}\int_\pi^{2\pi}1\ dx=1$ \\
$\displaystyle a_k=\frac{1}{\pi}\int_0^{2\pi}f(x)\cos kx\ dx=\frac{1}{\pi}\int_\pi^{2\pi}\cos kx\ dx=\frac{1}{\pi}\left.\frac{\sin kx}{k}\right|_\pi^{2\pi}=0$ \\
$\displaystyle b_k=\frac{1}{\pi}\int_0^{2\pi}f(x)\sin kx\ dx=\frac{1}{\pi}\int_\pi^{2\pi}\sin kx\ dx=\frac{1}{\pi}\left.\frac{-\cos kx}{k}\right|_\pi^{2\pi}=\frac{1}{\pi}(-\frac{1}{k}-\frac{1}{k})=-\frac{2}{k\pi}$ \\
$\displaystyle f(x)=\frac{a_0}{2}+\sum_{k=1}^\infty(a_k\cos kx+b_k\sin kx)=\frac{1}{2}-\sum_{k=1}^\infty\frac{2\sin kx}{k\pi}$
\end{minipage}\\

\end{CJK}
\end{document}