\documentclass[12pt]{book}
\usepackage[utf8]{inputenc}
\usepackage{color,soul,CJK,epic,tikz,array}
\usepackage{amsmath,amsthm,amssymb}
\setlength{\parindent}{0em}
\linespread{1.3}
\author{andersonwu2000}

\textwidth=16.6cm
\textheight=23cm
\parindent=16pt
\oddsidemargin=-1.0cm
\evensidemargin=-1.0cm
\topmargin=-0.5cm

\newcounter{sect}

\newcounter{block}[sect]
\newenvironment{tblock}[1]
{\refstepcounter{block}\theblock.~\begin{minipage}[t]{\dimexpr\linewidth}#1\\}
{\end{minipage}\\}

\newenvironment{comm}
{\makebox[12pt][l]{$\bullet$}\begin{minipage}[t]{\dimexpr\linewidth}}
{\end{minipage}}

\newenvironment{code}
{\begin{minipage}[t]{\dimexpr\linewidth}\ttfamily }
{\end{minipage}}

\begin{document}
\begin{CJK}{UTF8}{bsmi}

%%--------------------------------------------
%%--------------------------------------------

% $\displaystyle H_n^{(m)}=\sum_{k=1}^n\frac{1}{k^m}$ \\
% $\displaystyle H_n^m=(H_n^{(1)})^m$ \\
% $\displaystyle \zeta(s) = \sum_{n=1}^\infty\frac{1}{n^s}$ \\
% $\displaystyle O_n^{(m)} = \sum_{k=1}^n\frac{1}{(2k-1)^m}$ \\
% $\displaystyle \overline{O}_n^{(m)} = \sum_{k=1}^n\frac{(-1)^{k-1}}{(2k-1)^m}$ \\
% $\displaystyle G=\sum^\infty_{n=1}\frac{(-1)^{n+1}}{(2n-1)^2}$ \\\\

$\pi = 3.141592653589793$ \\
$\ln(2) = 0.6931471805599453$ \\
$G = 0.915965594177219$ \\
$\zeta(3)=1.2020569031595942$ \\

$$\begin{array}{|l|rlc|}
\hline
\text{no.} & 
\text{formula\qquad\qquad\qquad} & 
\text{value in }10^8 \text{ terms} & 
\text{correct} \\
\hline
1 & \displaystyle\sum_{n=0}^\infty\frac{H^{(2)}_{4n}}{(2n+1)(2n+5)}= &
0.\underline{20358293}254907192 & 8 \\
&n\displaystyle-\frac{13G}{315}+\frac{5473\pi^2}{161280}+\frac{491\pi}{99225}+\frac{36881\ln(2)}{793800}-\frac{42058}{297675}= &
0.\underline{20358293}65950119 & \\[5pt]
\hline
2 & \displaystyle \sum_{n=0}^\infty\frac{(-1)^nH_{2n}^2}{(n+1)(n+3)}= &
-0.\underline{1275118080691}6856 & 13\\
& \displaystyle -\frac{2G}{15}-\frac{97\pi^2}{960}+\frac{247\pi}{450}+\frac{\pi\ln(2)}{30}+\frac{23\ln^2(2)}{60}-\frac{572\ln(2)}{225}+\frac{11129}{14400}= &
-0.\underline{1275118080691}5474 & \\[5pt]
\hline
3 & \displaystyle \sum_{n=0}^\infty\frac{H_n^{(2)}}{(2n+1)(2n+5)}= &
0.\underline{1703267}3737748197 & 7 \\
 & \displaystyle \frac{\pi^2}{18}+\frac{10\ln(2)}{9}-\frac{31}{27}= &
0.\underline{1703267}414234222 & \\[5pt]
\hline
4 & \displaystyle \sum_{n=0}^\infty\frac{H_n^2}{(2n+1)(2n+5)}= &
0.\underline{67484}48211374997 & 5 \\
 & \displaystyle \frac{4\ln^2(2)}{3}-\frac{16\ln(2)}{9}-\frac{\pi^2}{18}+\frac{49}{27}= &
0.\underline{67484}58234275496 & \\[5pt]
\hline
5 & \displaystyle \sum_{n=0}^\infty\frac{H_{2n}^2}{(n+1)(n+3)}= &
3.\underline{67601}4246104275 & 5 \\
 & \displaystyle \frac{47\pi^2}{480}-\frac{8\ln^2(2)}{15}+\frac{679\ln(2)}{225}+\frac{12587}{14400}= &
3.\underline{67601}85372956378 & \\[5pt]
\hline
6 & \displaystyle \sum_{n=0}^\infty\frac{(-1)^nH_{2n}^{(2)}}{(n+1)(n+3)}= &
-0.\underline{09820503952207}756 & 14 \\
 & \displaystyle -\frac{2G}{15}-\frac{\pi^2}{192}+\frac{4\pi}{225}+\frac{293\ln(2)}{900}-\frac{2969}{14400}= &
-0.\underline{09820503952207}998 & \\[5pt]
\hline
7 & \displaystyle \sum_{n=0}^\infty\frac{\overline{O}_n^{(2)}}{(n+1)(n+2)}= &
0.\underline{4702055}528500617 & 7 \\
 & \displaystyle \frac{1}{9}+\frac{2G}{3}-\frac{\pi}{18}-\frac{\ln(2)}{9}= &
0.\underline{4702055}61967608 & \\[5pt]
\hline
\end{array}$$
$$\begin{array}{|l|rlc|}
\hline
\text{no.} & 
\text{formula\qquad\qquad\qquad} & 
\text{value in }10^8 \text{ terms} & 
\text{correct} \\
8 & \displaystyle \sum_{n=0}^\infty\frac{O_n^{(2)}}{(n+1)(n+2)}= &
0.\underline{5573232}029937555 & 7 \\
 & \displaystyle \frac{3\pi^2-8\ln(2)-4}{36}= &
0.\underline{5573232}155219031 & \\[5pt]
\hline
9 & \displaystyle \sum_{n=0}^\infty\frac{H_{2n}^{(2)}}{(n+1)(n+2)}= &
0.\underline{7185567}160501689 & 7 \\
 & \displaystyle \frac{\pi^2}{8}-\frac{2\ln(2)}{9}-\frac{13}{36}= &
0.\underline{7185567}322339597 & \\[5pt]
\hline
10 & \displaystyle \sum_{n=0}^\infty\frac{H_{2n}^{(2)}}{(n+1)(n+3)}= &
0.\underline{6042259}519160843 & 7 \\
 & \displaystyle \frac{47\pi^2}{480}-\frac{34\ln(2)}{225}-\frac{3707}{14400}= &
0.\underline{6042259}680998301 & \\[5pt]
\hline
11 & \displaystyle \sum_{n=0}^\infty\frac{H_{2n}^{2}}{(n+1)(n+2)}= &
4.\underline{07236}2002785773 & 5 \\
 & \displaystyle \frac{\pi^2}{8}+\frac{32\ln(2)}{9}-\frac{2\ln^2(2)}{3}+\frac{25}{36}= &
4.\underline{07236}6293959397 & \\[5pt]
\hline
12 & \displaystyle \sum_{n=0}^\infty\frac{H_{n}^{2}}{(2n+1)(2n+13)}= &
0.\underline{51707}44439107315 & 5 \\
 & \displaystyle \frac{6508\ln^2(2)}{10395}-\frac{42354064\ln(2)}{36018675}-\frac{1627\pi^2}{62370}+\frac{160848964597}{124804708875}= &
0.\underline{51707}54462007356 & \\[5pt]
\hline
13 & \displaystyle \sum_{n=0}^\infty\frac{H_{2n}^{(2)}}{(2n+1)(2n+3)}= &
0.\underline{23561548}212410635 & 8 \\
 & \displaystyle \frac{5\pi^2}{96} + \frac{\ln(2)}{2} - \frac{5}{8}= &
0.\underline{23561548}617004346 & \\[5pt]
\hline
14 & \displaystyle \sum_{n=0}^\infty\frac{H_{n}^{2}}{(2n+1)(2n+3)}= &
0.\underline{75214363}10023859 & 8 \\
 & \displaystyle 2-\frac{\pi^2}{12}-2\ln(2)+2\ln^2(2)= &
0.\underline{75214463}32923989 & \\[5pt]
\hline
15 & \displaystyle \sum_{n=0}^\infty\frac{H_{n}^{2}}{(2n+1)(2n+7)}= &
0.\underline{62026}32980158675 & 5 \\
 & \displaystyle \frac{46\ln^2(2)}{45}-\frac{1058\ln(2)}{675}-\frac{23\pi^2}{540}+\frac{16564}{10125}= &
0.\underline{62026}4300305903 & \\[5pt]
\hline
16 & \displaystyle \sum_{n=0}^\infty\frac{H_{n}^{2}}{(2n+1)(2n+9)}= &
0.\underline{578}4990173844122 & 3 \\
 & \displaystyle \frac{88\ln^2(2)}{105}-\frac{15488\ln(2)}{11025}-\frac{11\pi^2}{315}+\frac{1729753}{1157625}=  &
0.\underline{578}5000196744163 & \\[5pt]
\hline
17 & \displaystyle \sum_{n=0}^\infty\frac{H_{n}^{2}}{(2n+1)(2n+11)}= &
0.\underline{54494}26841432881 & 5 \\
 & \displaystyle \frac{1126\ln^2(2)}{1575}-\frac{633938\ln(2)}{496125}-\frac{563\pi^2}{18900}+\frac{215844634}{156279375}= &
0.\underline{54494}36864332522 & \\[5pt]
\hline
\end{array}$$
$$\begin{array}{|l|rlc|}
\hline
\text{no.} & 
\text{formula\qquad\qquad\qquad} & 
\text{value in }10^8 \text{ terms} & 
\text{correct} \\
18 & \displaystyle \sum_{n=0}^\infty\frac{H_{4n}^{(2)}}{(2n+1)(2n+3)}= &
0.\underline{25301046}019292905 & 8 \\
 & \displaystyle -\frac{G}{15}+\frac{89\pi^2}{1920}+\frac{2\pi}{225}+\frac{157\ln(2)}{1800}-\frac{1669}{7200}= &
0.\underline{25301046}4288875 & \\[5pt]
\hline
19 & \displaystyle \sum_{n=0}^\infty\frac{H_{n}^{2}}{(n+1)(2n+1)}= &
1.\underline{61284}31706704522 & 5 \\
 & \displaystyle \frac{5\zeta(3)}{2}-\frac{\pi^2\ln(2)}{3}+\frac{8\ln^3(2)}{3}= &
1.\underline{61284}51752504258 & \\[5pt]
\hline
20 & \displaystyle \sum_{n=0}^\infty\frac{H_{2n}^{(2)}}{(2n+1)(2n+5)}= &
0.\underline{19056720}112710754 & 8 \\
 & \displaystyle \frac{43\pi^2}{1152}+\frac{5\ln(2)}{18}-\frac{10}{27}= &
0.\underline{19056720}517305403 & \\[5pt]
\hline
21 & \displaystyle \sum_{n=0}^\infty\frac{H_{2n}^{2}}{(2n+1)(2n+5)}= &
1.\underline{04509}58110109523 & 5 \\
 & \displaystyle \frac{43\pi^2}{1152}+\frac{\ln^2(2)}{3}-\frac{31\ln(2)}{36}+\frac{481}{432}= &
1.\underline{04509}68838043684 & \\[5pt]
\hline
22 & \displaystyle \sum_{n=0}^\infty\frac{H_{4n}^{2}}{(2n+1)(2n+3)}= &
1.\underline{77425}22188998273 & 5 \\
 & \displaystyle -\frac{G}{15}-\frac{\pi^2}{640}+\frac{247\pi}{900}+\frac{\pi\ln(2)}{60}-\frac{3\ln^2(2)}{40}-\frac{107\ln(2)}{450}+\frac{5929}{7200}= &
1.\underline{77425}3364613242 & \\[5pt]
\hline
23 & \displaystyle \sum_{n=0}^\infty\frac{H_{2n}^{(2)}}{(n+1)(n+2)(n+3)}= &
0.\underline{11433076413}240427 & 11 \\
 & \displaystyle \frac{13\pi^2}{480}+\frac{16\ln(2)}{225}-\frac{1493}{14400}= & 
0.\underline{11433076413}412954 & \\[5pt]
24 & \displaystyle \sum_{n=0}^\infty\frac{H_{2n}^2}{(n+1)(n+2)(n+3)}= &
0.\underline{3963477566}3891836 & 10 \\
 & \displaystyle \frac{13\pi^2}{480}+\frac{121\ln(2)}{225}-\frac{2\ln^2(2)}{15}-\frac{2587}{14400}= & 
0.\underline{3963477566}637582 & \\[5pt]
\hline
25 & \displaystyle \sum_{n=0}^\infty\frac{H_{2n}^2}{(2n+1)(2n+3)}= &
1.\underline{18612}01494958684 & 5 \\
 & \displaystyle \frac{5\pi^2}{96}+\frac{\ln^2(2)}{2}-\ln(2)+\frac{9}{8}= &
1.\underline{18612}12222892261 & \\[5pt]
\hline
26 & \displaystyle \sum_{n=0}^\infty\frac{H_{2n}^{(2)}+H_{2n}^{2}}{(n+1)(n+2)}= &
4.\underline{7909}18718520726 & 4 \\
 & \displaystyle \frac{\pi^2}{4}+\frac{10\ln(2)}{3}-\frac{2\ln^2(2)}{3}+\frac{1}{3}= & 
4.\underline{7909}23026193356 \\[5pt]
\hline
27 & \displaystyle \sum_{n=0}^\infty\frac{H_n^{(2)}}{(n+1)(2n+1)}= &
0.\underline{4772774}584544363 & 7 \\
 & \displaystyle \frac{\pi^2\ln(2)}{3}-\frac{3\zeta(3)}{2}= &
0.\underline{4772774}6654631353 \\[5pt]
\hline
\end{array}$$



\end{CJK}
\end{document}